Let axioms decide if they can be hidden

Source/DafnyCore/Verifier/BoogieGenerator.Functions.cs
@@ -813,7 +813,6 @@ public partial class BoogieGenerator {
         RequiresName(f), new List<Bpl.TypeVariable>(),
         funcFormals.ConvertAll(v => (Bpl.Variable)BplFormalVar(null, v.TypedIdent.Type, true)),
         BplFormalVar(null, Bpl.Type.Bool, false));
-      precondF.AlwaysRevealed = true;
       sink.AddTopLevelDeclaration(precondF);
 
       var appl = FunctionCall(f.tok, RequiresName(f), Bpl.Type.Bool, reqFuncArguments);
@@ -914,7 +913,9 @@ public partial class BoogieGenerator {
     } else {
       comment += " (opaque)";
     }
-    return new Axiom(f.tok, BplImp(activate, ax), comment);
+    return new Axiom(f.tok, BplImp(activate, ax), comment) {
+      CanHide = true
+    };
   }
 
 
