Source/DafnyCore/DafnyPrelude.bpl
@@ -34,51 +34,51 @@ const unique TORDINAL  : Ty uses {
   axiom Tag(TORDINAL) == TagORDINAL;
 }
 // See for which axioms we can make use of the trigger to determine the connection.
-revealed function TBitvector(int) : Ty;
+function TBitvector(int) : Ty;
 axiom (forall w: int :: { TBitvector(w) } Inv0_TBitvector(TBitvector(w)) == w);
 
-revealed function TSet(Ty) : Ty;
+function TSet(Ty) : Ty;
 axiom (forall t: Ty :: { TSet(t) } Inv0_TSet(TSet(t)) == t);
 axiom (forall t: Ty :: { TSet(t) }      Tag(TSet(t))      == TagSet);
 
-revealed function TISet(Ty) : Ty;
+function TISet(Ty) : Ty;
 axiom (forall t: Ty :: { TISet(t) } Inv0_TISet(TISet(t)) == t);
 axiom (forall t: Ty :: { TISet(t) }     Tag(TISet(t))     == TagISet);
 
-revealed function TMultiSet(Ty) : Ty;
+function TMultiSet(Ty) : Ty;
 axiom (forall t: Ty :: { TMultiSet(t) } Inv0_TMultiSet(TMultiSet(t)) == t);
 axiom (forall t: Ty :: { TMultiSet(t) } Tag(TMultiSet(t)) == TagMultiSet);
 
-revealed function TSeq(Ty) : Ty;
+function TSeq(Ty) : Ty;
 axiom (forall t: Ty :: { TSeq(t) } Inv0_TSeq(TSeq(t)) == t);
 axiom (forall t: Ty :: { TSeq(t) } Tag(TSeq(t)) == TagSeq);
 
-revealed function TMap(Ty, Ty) : Ty;
+function TMap(Ty, Ty) : Ty;
 axiom (forall t, u: Ty :: { TMap(t,u) } Inv0_TMap(TMap(t,u)) == t);
 axiom (forall t, u: Ty :: { TMap(t,u) } Inv1_TMap(TMap(t,u)) == u);
 axiom (forall t, u: Ty :: { TMap(t,u) } Tag(TMap(t,u)) == TagMap);
 
-revealed function TIMap(Ty, Ty) : Ty;
+function TIMap(Ty, Ty) : Ty;
 axiom (forall t, u: Ty :: { TIMap(t,u) } Inv0_TIMap(TIMap(t,u)) == t);
 axiom (forall t, u: Ty :: { TIMap(t,u) } Inv1_TIMap(TIMap(t,u)) == u);
 axiom (forall t, u: Ty :: { TIMap(t,u) } Tag(TIMap(t,u)) == TagIMap);
 
 
-revealed function Inv0_TBitvector(Ty) : int;
-revealed function Inv0_TSet(Ty) : Ty;
-revealed function Inv0_TISet(Ty) : Ty;
-revealed function Inv0_TSeq(Ty) : Ty;
-revealed function Inv0_TMultiSet(Ty) : Ty;
-revealed function Inv0_TMap(Ty) : Ty;
-revealed function Inv1_TMap(Ty) : Ty;
-revealed function Inv0_TIMap(Ty) : Ty;
-revealed function Inv1_TIMap(Ty) : Ty;
+function Inv0_TBitvector(Ty) : int;
+function Inv0_TSet(Ty) : Ty;
+function Inv0_TISet(Ty) : Ty;
+function Inv0_TSeq(Ty) : Ty;
+function Inv0_TMultiSet(Ty) : Ty;
+function Inv0_TMap(Ty) : Ty;
+function Inv1_TMap(Ty) : Ty;
+function Inv0_TIMap(Ty) : Ty;
+function Inv1_TIMap(Ty) : Ty;
 
 // -- Classes and Datatypes --
 
 // -- Type Tags --
 type TyTag;
-revealed function Tag(Ty) : TyTag;
+function Tag(Ty) : TyTag;
 
 const unique TagBool     : TyTag;
 const unique TagChar     : TyTag;
@@ -94,21 +94,21 @@ const unique TagIMap     : TyTag;
 const unique TagClass    : TyTag;
 
 type TyTagFamily;
-revealed function TagFamily(Ty): TyTagFamily;
+function TagFamily(Ty): TyTagFamily;
 
 // ---------------------------------------------------------------
 // -- Literals ---------------------------------------------------
 // ---------------------------------------------------------------
-revealed function {:identity} Lit<T>(x: T): T { x }
+function {:identity} Lit<T>(x: T): T { x }
 axiom (forall<T> x: T :: { $Box(Lit(x)) } $Box(Lit(x)) == Lit($Box(x)) );
 
 // Specialize Lit to concrete types.
 // These aren't logically required, but on some examples improve
 // verification speed
-revealed function {:identity} LitInt(x: int): int { x }
+function {:identity} LitInt(x: int): int { x }
 axiom (forall x: int :: { $Box(LitInt(x)) } $Box(LitInt(x)) == Lit($Box(x)) );
 
-revealed function {:identity} LitReal(x: real): real { x }
+function {:identity} LitReal(x: real): real { x }
 axiom (forall x: real :: { $Box(LitReal(x)) } $Box(LitReal(x)) == Lit($Box(x)) );
 
 // ---------------------------------------------------------------
@@ -116,34 +116,34 @@ axiom (forall x: real :: { $Box(LitReal(x)) } $Box(LitReal(x)) == Lit($Box(x)) )
 // ---------------------------------------------------------------
 
 #if UNICODE_CHAR
-revealed function {:inline} char#IsChar(n: int): bool {
+function {:inline} char#IsChar(n: int): bool {
   (0                  <= n && n < 55296   /* 0xD800 */) || 
   (57344 /* 0xE000 */ <= n && n < 1114112 /* 0x11_0000 */ )
 }
 #else
-revealed function {:inline} char#IsChar(n: int): bool {
+function {:inline} char#IsChar(n: int): bool {
   0 <= n && n < 65536
 }
 #endif
 
 type char;
-revealed function char#FromInt(int): char;
+function char#FromInt(int): char;
 axiom (forall n: int ::
   { char#FromInt(n) }
   char#IsChar(n) ==> char#ToInt(char#FromInt(n)) == n);
 
-revealed function char#ToInt(char): int;
+function char#ToInt(char): int;
 axiom (forall ch: char ::
   { char#ToInt(ch) }
   char#FromInt(char#ToInt(ch)) == ch &&
   char#IsChar(char#ToInt(ch)));
 
-revealed function char#Plus(char, char): char;
+function char#Plus(char, char): char;
 axiom (forall a: char, b: char ::
   { char#Plus(a, b) }
   char#Plus(a, b) == char#FromInt(char#ToInt(a) + char#ToInt(b)));
 
-revealed function char#Minus(char, char): char;
+function char#Minus(char, char): char;
 axiom (forall a: char, b: char ::
   { char#Minus(a, b) }
   char#Minus(a, b) == char#FromInt(char#ToInt(a) - char#ToInt(b)));
@@ -162,16 +162,16 @@ const null: ref;
 type Box;
 const $ArbitraryBoxValue: Box;
 
-revealed function $Box<T>(T): Box;
-revealed function $Unbox<T>(Box): T;
+function $Box<T>(T): Box;
+function $Unbox<T>(Box): T;
 axiom (forall<T> x : T   :: { $Box(x) } $Unbox($Box(x)) == x);
 axiom (forall<T> x : Box :: { $Unbox(x): T} $Box($Unbox(x): T) == x);
 
 
 // Corresponding entries for boxes...
 // This could probably be solved by having Box also inhabit Ty
-revealed function $IsBox(Box,Ty): bool;
-revealed function $IsAllocBox(Box,Ty,Heap): bool;
+function $IsBox(Box,Ty): bool;
+function $IsAllocBox(Box,Ty,Heap): bool;
 
 axiom (forall bx : Box ::
     { $IsBox(bx, TInt) }
@@ -224,7 +224,7 @@ axiom (forall<T> v : T, t : Ty, h : Heap ::
 
 // Type-argument to $Is is the /representation type/,
 // the second value argument to $Is is the actual type.
-revealed function $Is<T>(T,Ty): bool;           // no heap for now
+function $Is<T>(T,Ty): bool;           // no heap for now
 axiom(forall v : int  :: { $Is(v,TInt) }  $Is(v,TInt));
 axiom(forall v : real :: { $Is(v,TReal) } $Is(v,TReal));
 axiom(forall v : bool :: { $Is(v,TBool) } $Is(v,TBool));
@@ -285,7 +285,7 @@ axiom (forall v: IMap, t0: Ty, t1: Ty ::
     $Is(IMap#Values(v), TISet(t1)) &&
     $Is(IMap#Items(v), TISet(Tclass._System.Tuple2(t0, t1))));
 
-revealed function $IsAlloc<T>(T,Ty,Heap): bool;
+function $IsAlloc<T>(T,Ty,Heap): bool;
 axiom(forall h : Heap, v : int  :: { $IsAlloc(v,TInt,h) }  $IsAlloc(v,TInt,h));
 axiom(forall h : Heap, v : real :: { $IsAlloc(v,TReal,h) } $IsAlloc(v,TReal,h));
 axiom(forall h : Heap, v : bool :: { $IsAlloc(v,TBool,h) } $IsAlloc(v,TBool,h));
@@ -331,12 +331,12 @@ axiom (forall v: IMap, t0: Ty, t1: Ty, h: Heap ::
         $IsAllocBox(bx, t0, h)));
 
 
-revealed function $AlwaysAllocated(Ty): bool;
+function $AlwaysAllocated(Ty): bool;
   axiom (forall ty: Ty :: { $AlwaysAllocated(ty) }
     $AlwaysAllocated(ty) ==>
     (forall h: Heap, v: Box  :: { $IsAllocBox(v, ty, h) }  $IsBox(v, ty) ==> $IsAllocBox(v, ty, h)));
 
-revealed function $OlderTag(Heap): bool;
+function $OlderTag(Heap): bool;
 
 // ---------------------------------------------------------------
 // -- Encoding of type names -------------------------------------
@@ -349,14 +349,14 @@ const unique class._System.set: ClassName;
 const unique class._System.seq: ClassName;
 const unique class._System.multiset: ClassName;
 
-revealed function Tclass._System.object?(): Ty;
-revealed function Tclass._System.Tuple2(Ty, Ty): Ty;
+function Tclass._System.object?(): Ty;
+function Tclass._System.Tuple2(Ty, Ty): Ty;
 
-revealed function /*{:never_pattern true}*/ dtype(ref): Ty; // changed from ClassName to Ty
+function /*{:never_pattern true}*/ dtype(ref): Ty; // changed from ClassName to Ty
 
-revealed function TypeTuple(a: ClassName, b: ClassName): ClassName;
-revealed function TypeTupleCar(ClassName): ClassName;
-revealed function TypeTupleCdr(ClassName): ClassName;
+function TypeTuple(a: ClassName, b: ClassName): ClassName;
+function TypeTupleCar(ClassName): ClassName;
+function TypeTupleCdr(ClassName): ClassName;
 // TypeTuple is injective in both arguments:
 axiom (forall a: ClassName, b: ClassName :: { TypeTuple(a,b) }
   TypeTupleCar(TypeTuple(a,b)) == a &&
@@ -366,7 +366,7 @@ axiom (forall a: ClassName, b: ClassName :: { TypeTuple(a,b) }
 
 type HandleType;
 
-revealed function SetRef_to_SetBox(s: [ref]bool): Set;
+function SetRef_to_SetBox(s: [ref]bool): Set;
 axiom (forall s: [ref]bool, bx: Box :: { SetRef_to_SetBox(s)[bx] }
   SetRef_to_SetBox(s)[bx] == s[$Unbox(bx): ref]);
 axiom (forall s: [ref]bool :: { SetRef_to_SetBox(s) }
@@ -374,7 +374,7 @@ axiom (forall s: [ref]bool :: { SetRef_to_SetBox(s) }
 
 // Functions ApplyN, RequiresN, and ReadsN are generated on demand by the translator,
 // but Apply1 is referred to in the prelude, so its definition is hardcoded here.
-revealed function Apply1(Ty, Ty, Heap, HandleType, Box): Box;
+function Apply1(Ty, Ty, Heap, HandleType, Box): Box;
 
 // ---------------------------------------------------------------
 // -- Datatypes --------------------------------------------------
@@ -383,10 +383,10 @@ revealed function Apply1(Ty, Ty, Heap, HandleType, Box): Box;
 type DatatypeType;
 
 type DtCtorId;
-revealed function DatatypeCtorId(DatatypeType): DtCtorId;
+function DatatypeCtorId(DatatypeType): DtCtorId;
 
-revealed function DtRank(DatatypeType): int;
-revealed function BoxRank(Box): int;
+function DtRank(DatatypeType): int;
+function BoxRank(Box): int;
 
 axiom (forall d: DatatypeType :: {BoxRank($Box(d))} BoxRank($Box(d)) == DtRank(d));
 
@@ -401,20 +401,20 @@ type ORDINAL = Box;  // :| There are more big ordinals than boxes
 // numbers.  Function ORD#Offset gives how many successors (that is,
 // +1 operations) an ordinal is above the nearest lower limit ordinal.
 // That is, if the ordinal is \lambda+n, then ORD#Offset returns n.
-revealed function ORD#IsNat(ORDINAL): bool;
-revealed function ORD#Offset(ORDINAL): int;
+function ORD#IsNat(ORDINAL): bool;
+function ORD#Offset(ORDINAL): int;
 axiom (forall o:ORDINAL :: { ORD#Offset(o) } 0 <= ORD#Offset(o));
 
-revealed function {:inline} ORD#IsLimit(o: ORDINAL): bool { ORD#Offset(o) == 0 }
-revealed function {:inline} ORD#IsSucc(o: ORDINAL): bool { 0 < ORD#Offset(o) }
+function {:inline} ORD#IsLimit(o: ORDINAL): bool { ORD#Offset(o) == 0 }
+function {:inline} ORD#IsSucc(o: ORDINAL): bool { 0 < ORD#Offset(o) }
 
-revealed function ORD#FromNat(int): ORDINAL;
+function ORD#FromNat(int): ORDINAL;
 axiom (forall n:int :: { ORD#FromNat(n) }
   0 <= n ==> ORD#IsNat(ORD#FromNat(n)) && ORD#Offset(ORD#FromNat(n)) == n);
 axiom (forall o:ORDINAL :: { ORD#Offset(o) } { ORD#IsNat(o) }
   ORD#IsNat(o) ==> o == ORD#FromNat(ORD#Offset(o)));
 
-revealed function ORD#Less(ORDINAL, ORDINAL): bool;
+function ORD#Less(ORDINAL, ORDINAL): bool;
 axiom (forall o,p: ORDINAL :: { ORD#Less(o,p) }
   (ORD#Less(o,p) ==> o != p) &&  // irreflexivity
   (ORD#IsNat(o) && !ORD#IsNat(p) ==> ORD#Less(o,p)) &&
@@ -430,11 +430,11 @@ axiom (forall o,p,r: ORDINAL ::
   ORD#Less(o,p) && ORD#Less(p,r) ==> ORD#Less(o,r));
 
 // ORD#LessThanLimit is a synonym of ORD#Less, introduced for more selected triggering
-revealed function ORD#LessThanLimit(ORDINAL, ORDINAL): bool;
+function ORD#LessThanLimit(ORDINAL, ORDINAL): bool;
 axiom (forall o,p: ORDINAL :: { ORD#LessThanLimit(o, p) }
   ORD#LessThanLimit(o, p) == ORD#Less(o, p));
 
-revealed function ORD#Plus(ORDINAL, ORDINAL): ORDINAL;
+function ORD#Plus(ORDINAL, ORDINAL): ORDINAL;
 axiom (forall o,p: ORDINAL :: { ORD#Plus(o,p) }
   (ORD#IsNat(ORD#Plus(o,p)) ==> ORD#IsNat(o) && ORD#IsNat(p)) &&
   (ORD#IsNat(p) ==>
@@ -447,7 +447,7 @@ axiom (forall o,p: ORDINAL :: { ORD#Plus(o,p) }
   (o == ORD#FromNat(0) ==> ORD#Plus(o, p) == p) &&
   (p == ORD#FromNat(0) ==> ORD#Plus(o, p) == o));
 
-revealed function ORD#Minus(ORDINAL, ORDINAL): ORDINAL;
+function ORD#Minus(ORDINAL, ORDINAL): ORDINAL;
 axiom (forall o,p: ORDINAL :: { ORD#Minus(o,p) }
   ORD#IsNat(p) && ORD#Offset(p) <= ORD#Offset(o) ==>
     ORD#IsNat(ORD#Minus(o,p)) == ORD#IsNat(o) &&
@@ -494,10 +494,10 @@ const $FunctionContextHeight: int;
 
 type LayerType;
 const $LZ: LayerType;
-revealed function $LS(LayerType): LayerType;
-revealed function AsFuelBottom(LayerType) : LayerType;
+function $LS(LayerType): LayerType;
+function AsFuelBottom(LayerType) : LayerType;
 
-revealed function AtLayer<A>([LayerType]A, LayerType): A;
+function AtLayer<A>([LayerType]A, LayerType): A;
 axiom (forall<A> f : [LayerType]A, ly : LayerType :: { AtLayer(f,ly) } AtLayer(f,ly) == f[ly]);
 axiom (forall<A> f : [LayerType]A, ly : LayerType :: { AtLayer(f,$LS(ly)) } AtLayer(f,$LS(ly)) == AtLayer(f,ly));
 
@@ -507,35 +507,35 @@ axiom (forall<A> f : [LayerType]A, ly : LayerType :: { AtLayer(f,$LS(ly)) } AtLa
 
 type Field;
 
-revealed function FDim(Field): int uses {
+function FDim(Field): int uses {
   axiom FDim(alloc) == 0;
 }
 
-revealed function IndexField(int): Field;
+function IndexField(int): Field;
 axiom (forall i: int :: { IndexField(i) } FDim(IndexField(i)) == 1);
-revealed function IndexField_Inverse(Field): int;
+function IndexField_Inverse(Field): int;
 axiom (forall i: int :: { IndexField(i) } IndexField_Inverse(IndexField(i)) == i);
 
-revealed function MultiIndexField(Field, int): Field;
+function MultiIndexField(Field, int): Field;
 axiom (forall f: Field, i: int :: { MultiIndexField(f,i) } FDim(MultiIndexField(f,i)) == FDim(f) + 1);
-revealed function MultiIndexField_Inverse0(Field): Field;
-revealed function MultiIndexField_Inverse1(Field): int;
+function MultiIndexField_Inverse0(Field): Field;
+function MultiIndexField_Inverse1(Field): int;
 axiom (forall f: Field, i: int :: { MultiIndexField(f,i) }
   MultiIndexField_Inverse0(MultiIndexField(f,i)) == f &&
   MultiIndexField_Inverse1(MultiIndexField(f,i)) == i);
 
-revealed function DeclType(Field): ClassName;
+function DeclType(Field): ClassName;
 
 type NameFamily;
-revealed function DeclName(Field): NameFamily uses {
+function DeclName(Field): NameFamily uses {
   axiom DeclName(alloc) == allocName;
 }
-revealed function FieldOfDecl(ClassName, NameFamily): Field;
+function FieldOfDecl(ClassName, NameFamily): Field;
 axiom (forall cl : ClassName, nm: NameFamily ::
    {FieldOfDecl(cl, nm): Field}
    DeclType(FieldOfDecl(cl, nm): Field) == cl && DeclName(FieldOfDecl(cl, nm): Field) == nm);
 
-revealed function $IsGhostField(Field): bool uses {
+function $IsGhostField(Field): bool uses {
    axiom $IsGhostField(alloc); // treat as ghost field, since it is allowed to be changed by ghost code
 }
 axiom (forall h: Heap, k: Heap :: { $HeapSuccGhost(h,k) }
@@ -567,7 +567,7 @@ const unique allocName: NameFamily;
 // -- Arrays -----------------------------------------------------
 // ---------------------------------------------------------------
 
-revealed function _System.array.Length(a: ref): int;
+function _System.array.Length(a: ref): int;
 axiom (forall o: ref :: {_System.array.Length(o)} 0 <= _System.array.Length(o));
 
 
@@ -575,21 +575,21 @@ axiom (forall o: ref :: {_System.array.Length(o)} 0 <= _System.array.Length(o));
 // -- Reals ------------------------------------------------------
 // ---------------------------------------------------------------
 
-revealed function Int(x: real): int { int(x) }
-revealed function Real(x: int): real { real(x) }
+function Int(x: real): int { int(x) }
+function Real(x: int): real { real(x) }
 axiom (forall i: int :: { Int(Real(i)) } Int(Real(i)) == i);
 
-revealed function {:inline} _System.real.Floor(x: real): int { Int(x) }
+function {:inline} _System.real.Floor(x: real): int { Int(x) }
 
 // ---------------------------------------------------------------
 // -- The heap ---------------------------------------------------
 // ---------------------------------------------------------------
 type Heap = [ref][Field]Box;
-revealed function {:inline} read(H: Heap, r: ref, f: Field) : Box { H[r][f] }
-revealed function {:inline} update(H:Heap, r:ref, f: Field, v: Box) : Heap { H[r := H[r][f := v]] }
+function {:inline} read(H: Heap, r: ref, f: Field) : Box { H[r][f] }
+function {:inline} update(H:Heap, r:ref, f: Field, v: Box) : Heap { H[r := H[r][f := v]] }
 
-revealed function $IsGoodHeap(Heap): bool;
-revealed function $IsHeapAnchor(Heap): bool;
+function $IsGoodHeap(Heap): bool;
+function $IsHeapAnchor(Heap): bool;
 var $Heap: Heap where $IsGoodHeap($Heap) && $IsHeapAnchor($Heap);
 
 // The following is used as a reference heap in places where the translation needs a heap
@@ -599,7 +599,7 @@ const $OneHeap: Heap uses {
   axiom $IsGoodHeap($OneHeap);
 }
 
-revealed function $HeapSucc(Heap, Heap): bool;
+function $HeapSucc(Heap, Heap): bool;
 axiom (forall h: Heap, r: ref, f: Field, x: Box :: { update(h, r, f, x) }
   $IsGoodHeap(update(h, r, f, x)) ==>
   $HeapSucc(h, update(h, r, f, x)));
@@ -608,7 +608,7 @@ axiom (forall a,b,c: Heap :: { $HeapSucc(a,b), $HeapSucc(b,c) }
 axiom (forall h: Heap, k: Heap :: { $HeapSucc(h,k) }
   $HeapSucc(h,k) ==> (forall o: ref :: { read(k, o, alloc) } $Unbox(read(h, o, alloc)) ==> $Unbox(read(k, o, alloc))));
 
-revealed function $HeapSuccGhost(Heap, Heap): bool;
+function $HeapSuccGhost(Heap, Heap): bool;
 
 // ---------------------------------------------------------------
 // -- Useful macros ----------------------------------------------
@@ -657,10 +657,10 @@ procedure $IterCollectNewObjects(prevHeap: Heap, newHeap: Heap, this: ref, NW: F
 
 type Set = [Box]bool;
 
-revealed function Set#Card(Set): int;
+function Set#Card(Set): int;
 axiom (forall s: Set :: { Set#Card(s) } 0 <= Set#Card(s));
 
-revealed function Set#Empty(): Set;
+function Set#Empty(): Set;
 axiom (forall o: Box :: { Set#Empty()[o] } !Set#Empty()[o]);
 axiom (forall s: Set :: { Set#Card(s) }
   (Set#Card(s) == 0 <==> s == Set#Empty()) &&
@@ -669,12 +669,12 @@ axiom (forall s: Set :: { Set#Card(s) }
 // the empty set could be of anything
 //axiom (forall t: Ty :: { $Is(Set#Empty() : [Box]bool, TSet(t)) } $Is(Set#Empty() : [Box]bool, TSet(t)));
 
-revealed function Set#Singleton(Box): Set;
+function Set#Singleton(Box): Set;
 axiom (forall r: Box :: { Set#Singleton(r) } Set#Singleton(r)[r]);
 axiom (forall r: Box, o: Box :: { Set#Singleton(r)[o] } Set#Singleton(r)[o] <==> r == o);
 axiom (forall r: Box :: { Set#Card(Set#Singleton(r)) } Set#Card(Set#Singleton(r)) == 1);
 
-revealed function Set#UnionOne(Set, Box): Set;
+function Set#UnionOne(Set, Box): Set;
 axiom (forall a: Set, x: Box, o: Box :: { Set#UnionOne(a,x)[o] }
   Set#UnionOne(a,x)[o] <==> o == x || a[o]);
 axiom (forall a: Set, x: Box :: { Set#UnionOne(a, x) }
@@ -686,7 +686,7 @@ axiom (forall a: Set, x: Box :: { Set#Card(Set#UnionOne(a, x)) }
 axiom (forall a: Set, x: Box :: { Set#Card(Set#UnionOne(a, x)) }
   !a[x] ==> Set#Card(Set#UnionOne(a, x)) == Set#Card(a) + 1);
 
-revealed function Set#Union(Set, Set): Set;
+function Set#Union(Set, Set): Set;
 axiom (forall a: Set, b: Set, o: Box :: { Set#Union(a,b)[o] }
   Set#Union(a,b)[o] <==> a[o] || b[o]);
 axiom (forall a, b: Set, y: Box :: { Set#Union(a, b), a[y] }
@@ -702,7 +702,7 @@ axiom (forall a, b: Set :: { Set#Union(a, b) }
 //   Set#Disjoint(a, b) ==>
 //     Set#Card(Set#Union(a, b)) == Set#Card(a) + Set#Card(b));
 
-revealed function Set#Intersection(Set, Set): Set;
+function Set#Intersection(Set, Set): Set;
 axiom (forall a: Set, b: Set, o: Box :: { Set#Intersection(a,b)[o] }
   Set#Intersection(a,b)[o] <==> a[o] && b[o]);
 
@@ -717,7 +717,7 @@ axiom (forall a, b: Set :: { Set#Intersection(a, Set#Intersection(a, b)) }
 axiom (forall a, b: Set :: { Set#Card(Set#Union(a, b)) }{ Set#Card(Set#Intersection(a, b)) }
   Set#Card(Set#Union(a, b)) + Set#Card(Set#Intersection(a, b)) == Set#Card(a) + Set#Card(b));
 
-revealed function Set#Difference(Set, Set): Set;
+function Set#Difference(Set, Set): Set;
 axiom (forall a: Set, b: Set, o: Box :: { Set#Difference(a,b)[o] }
   Set#Difference(a,b)[o] <==> a[o] && !b[o]);
 axiom (forall a, b: Set, y: Box :: { Set#Difference(a, b), b[y] }
@@ -729,7 +729,7 @@ axiom (forall a, b: Set ::
     == Set#Card(Set#Union(a, b)) &&
   Set#Card(Set#Difference(a, b)) == Set#Card(a) - Set#Card(Set#Intersection(a, b)));
 
-revealed function Set#Subset(Set, Set): bool;
+function Set#Subset(Set, Set): bool;
 axiom (forall a: Set, b: Set :: { Set#Subset(a,b) }
   Set#Subset(a,b) <==> (forall o: Box :: {a[o]} {b[o]} a[o] ==> b[o]));
 // axiom(forall a: Set, b: Set ::
@@ -737,13 +737,13 @@ axiom (forall a: Set, b: Set :: { Set#Subset(a,b) }
 //   Set#Subset(a,b) ==> Set#Card(a) <= Set#Card(b));
 
 
-revealed function Set#Equal(Set, Set): bool;
+function Set#Equal(Set, Set): bool;
 axiom (forall a: Set, b: Set :: { Set#Equal(a,b) }
   Set#Equal(a,b) <==> (forall o: Box :: {a[o]} {b[o]} a[o] <==> b[o]));
 axiom (forall a: Set, b: Set :: { Set#Equal(a,b) }  // extensionality axiom for sets
   Set#Equal(a,b) ==> a == b);
 
-revealed function Set#Disjoint(Set, Set): bool;
+function Set#Disjoint(Set, Set): bool;
 axiom (forall a: Set, b: Set :: { Set#Disjoint(a,b) }
   Set#Disjoint(a,b) <==> (forall o: Box :: {a[o]} {b[o]} !a[o] || !b[o]));
 
@@ -753,14 +753,14 @@ axiom (forall a: Set, b: Set :: { Set#Disjoint(a,b) }
 
 type ISet = [Box]bool;
 
-revealed function ISet#Empty(): Set;
+function ISet#Empty(): Set;
 axiom (forall o: Box :: { ISet#Empty()[o] } !ISet#Empty()[o]);
 
 // the empty set could be of anything
 //axiom (forall t: Ty :: { $Is(ISet#Empty() : [Box]bool, TISet(t)) } $Is(ISet#Empty() : [Box]bool, TISet(t)));
 
 
-revealed function ISet#UnionOne(ISet, Box): ISet;
+function ISet#UnionOne(ISet, Box): ISet;
 axiom (forall a: ISet, x: Box, o: Box :: { ISet#UnionOne(a,x)[o] }
   ISet#UnionOne(a,x)[o] <==> o == x || a[o]);
 axiom (forall a: ISet, x: Box :: { ISet#UnionOne(a, x) }
@@ -768,7 +768,7 @@ axiom (forall a: ISet, x: Box :: { ISet#UnionOne(a, x) }
 axiom (forall a: ISet, x: Box, y: Box :: { ISet#UnionOne(a, x), a[y] }
   a[y] ==> ISet#UnionOne(a, x)[y]);
 
-revealed function ISet#Union(ISet, ISet): ISet;
+function ISet#Union(ISet, ISet): ISet;
 axiom (forall a: ISet, b: ISet, o: Box :: { ISet#Union(a,b)[o] }
   ISet#Union(a,b)[o] <==> a[o] || b[o]);
 axiom (forall a, b: ISet, y: Box :: { ISet#Union(a, b), a[y] }
@@ -780,7 +780,7 @@ axiom (forall a, b: ISet :: { ISet#Union(a, b) }
     ISet#Difference(ISet#Union(a, b), a) == b &&
     ISet#Difference(ISet#Union(a, b), b) == a);
 
-revealed function ISet#Intersection(ISet, ISet): ISet;
+function ISet#Intersection(ISet, ISet): ISet;
 axiom (forall a: ISet, b: ISet, o: Box :: { ISet#Intersection(a,b)[o] }
   ISet#Intersection(a,b)[o] <==> a[o] && b[o]);
 
@@ -794,23 +794,23 @@ axiom (forall a, b: ISet :: { ISet#Intersection(a, ISet#Intersection(a, b)) }
   ISet#Intersection(a, ISet#Intersection(a, b)) == ISet#Intersection(a, b));
 
 
-revealed function ISet#Difference(ISet, ISet): ISet;
+function ISet#Difference(ISet, ISet): ISet;
 axiom (forall a: ISet, b: ISet, o: Box :: { ISet#Difference(a,b)[o] }
   ISet#Difference(a,b)[o] <==> a[o] && !b[o]);
 axiom (forall a, b: ISet, y: Box :: { ISet#Difference(a, b), b[y] }
   b[y] ==> !ISet#Difference(a, b)[y] );
 
-revealed function ISet#Subset(ISet, ISet): bool;
+function ISet#Subset(ISet, ISet): bool;
 axiom (forall a: ISet, b: ISet :: { ISet#Subset(a,b) }
   ISet#Subset(a,b) <==> (forall o: Box :: {a[o]} {b[o]} a[o] ==> b[o]));
 
-revealed function ISet#Equal(ISet, ISet): bool;
+function ISet#Equal(ISet, ISet): bool;
 axiom (forall a: ISet, b: ISet :: { ISet#Equal(a,b) }
   ISet#Equal(a,b) <==> (forall o: Box :: {a[o]} {b[o]} a[o] <==> b[o]));
 axiom (forall a: ISet, b: ISet :: { ISet#Equal(a,b) }  // extensionality axiom for sets
   ISet#Equal(a,b) ==> a == b);
 
-revealed function ISet#Disjoint(ISet, ISet): bool;
+function ISet#Disjoint(ISet, ISet): bool;
 axiom (forall a: ISet, b: ISet :: { ISet#Disjoint(a,b) }
   ISet#Disjoint(a,b) <==> (forall o: Box :: {a[o]} {b[o]} !a[o] || !b[o]));
 
@@ -818,40 +818,40 @@ axiom (forall a: ISet, b: ISet :: { ISet#Disjoint(a,b) }
 // -- Axiomatization of multisets --------------------------------
 // ---------------------------------------------------------------
 
-revealed function Math#min(a: int, b: int): int;
+function Math#min(a: int, b: int): int;
 axiom (forall a: int, b: int :: { Math#min(a, b) } a <= b <==> Math#min(a, b) == a);
 axiom (forall a: int, b: int :: { Math#min(a, b) } b <= a <==> Math#min(a, b) == b);
 axiom (forall a: int, b: int :: { Math#min(a, b) } Math#min(a, b) == a || Math#min(a, b) == b);
 
-revealed function Math#clip(a: int): int;
+function Math#clip(a: int): int;
 axiom (forall a: int :: { Math#clip(a) } 0 <= a ==> Math#clip(a) == a);
 axiom (forall a: int :: { Math#clip(a) } a < 0  ==> Math#clip(a) == 0);
 
 type MultiSet = [Box]int;
 
-revealed function $IsGoodMultiSet(ms: MultiSet): bool;
+function $IsGoodMultiSet(ms: MultiSet): bool;
 // ints are non-negative, used after havocing, and for conversion from sequences to multisets.
 axiom (forall ms: MultiSet :: { $IsGoodMultiSet(ms) }
   $IsGoodMultiSet(ms) <==>
   (forall bx: Box :: { ms[bx] } 0 <= ms[bx] && ms[bx] <= MultiSet#Card(ms)));
 
-revealed function MultiSet#Card(MultiSet): int;
+function MultiSet#Card(MultiSet): int;
 axiom (forall s: MultiSet :: { MultiSet#Card(s) } 0 <= MultiSet#Card(s));
 axiom (forall s: MultiSet, x: Box, n: int :: { MultiSet#Card(s[x := n]) }
   0 <= n ==> MultiSet#Card(s[x := n]) == MultiSet#Card(s) - s[x] + n);
 
-revealed function MultiSet#Empty(): MultiSet;
+function MultiSet#Empty(): MultiSet;
 axiom (forall o: Box :: { MultiSet#Empty()[o] } MultiSet#Empty()[o] == 0);
 axiom (forall s: MultiSet :: { MultiSet#Card(s) }
   (MultiSet#Card(s) == 0 <==> s == MultiSet#Empty()) &&
   (MultiSet#Card(s) != 0 ==> (exists x: Box :: 0 < s[x])));
 
-revealed function MultiSet#Singleton(Box): MultiSet;
+function MultiSet#Singleton(Box): MultiSet;
 axiom (forall r: Box, o: Box :: { MultiSet#Singleton(r)[o] } (MultiSet#Singleton(r)[o] == 1 <==> r == o) &&
                                                             (MultiSet#Singleton(r)[o] == 0 <==> r != o));
 axiom (forall r: Box :: { MultiSet#Singleton(r) } MultiSet#Singleton(r) == MultiSet#UnionOne(MultiSet#Empty(), r));
 
-revealed function MultiSet#UnionOne(MultiSet, Box): MultiSet;
+function MultiSet#UnionOne(MultiSet, Box): MultiSet;
 // pure containment axiom (in the original multiset or is the added element)
 axiom (forall a: MultiSet, x: Box, o: Box :: { MultiSet#UnionOne(a,x)[o] }
   0 < MultiSet#UnionOne(a,x)[o] <==> o == x || 0 < a[o]);
@@ -868,14 +868,14 @@ axiom (forall a: MultiSet, x: Box :: { MultiSet#Card(MultiSet#UnionOne(a, x)) }
   MultiSet#Card(MultiSet#UnionOne(a, x)) == MultiSet#Card(a) + 1);
 
 
-revealed function MultiSet#Union(MultiSet, MultiSet): MultiSet;
+function MultiSet#Union(MultiSet, MultiSet): MultiSet;
 // union-ing is the sum of the contents
 axiom (forall a: MultiSet, b: MultiSet, o: Box :: { MultiSet#Union(a,b)[o] }
   MultiSet#Union(a,b)[o] == a[o] + b[o]);
 axiom (forall a: MultiSet, b: MultiSet :: { MultiSet#Card(MultiSet#Union(a,b)) }
   MultiSet#Card(MultiSet#Union(a,b)) == MultiSet#Card(a) + MultiSet#Card(b));
 
-revealed function MultiSet#Intersection(MultiSet, MultiSet): MultiSet;
+function MultiSet#Intersection(MultiSet, MultiSet): MultiSet;
 axiom (forall a: MultiSet, b: MultiSet, o: Box :: { MultiSet#Intersection(a,b)[o] }
   MultiSet#Intersection(a,b)[o] == Math#min(a[o],  b[o]));
 
@@ -886,7 +886,7 @@ axiom (forall a, b: MultiSet :: { MultiSet#Intersection(a, MultiSet#Intersection
   MultiSet#Intersection(a, MultiSet#Intersection(a, b)) == MultiSet#Intersection(a, b));
 
 // multiset difference, a - b. clip() makes it positive.
-revealed function MultiSet#Difference(MultiSet, MultiSet): MultiSet;
+function MultiSet#Difference(MultiSet, MultiSet): MultiSet;
 axiom (forall a: MultiSet, b: MultiSet, o: Box :: { MultiSet#Difference(a,b)[o] }
   MultiSet#Difference(a,b)[o] == Math#clip(a[o] - b[o]));
 axiom (forall a, b: MultiSet, y: Box :: { MultiSet#Difference(a, b), b[y], a[y] }
@@ -899,23 +899,23 @@ axiom (forall a, b: MultiSet ::
   MultiSet#Card(MultiSet#Difference(a, b)) == MultiSet#Card(a) - MultiSet#Card(MultiSet#Intersection(a, b)));
 
 // multiset subset means a must have at most as many of each element as b
-revealed function MultiSet#Subset(MultiSet, MultiSet): bool;
+function MultiSet#Subset(MultiSet, MultiSet): bool;
 axiom (forall a: MultiSet, b: MultiSet :: { MultiSet#Subset(a,b) }
   MultiSet#Subset(a,b) <==> (forall o: Box :: {a[o]} {b[o]} a[o] <= b[o]));
 
-revealed function MultiSet#Equal(MultiSet, MultiSet): bool;
+function MultiSet#Equal(MultiSet, MultiSet): bool;
 axiom (forall a: MultiSet, b: MultiSet :: { MultiSet#Equal(a,b) }
   MultiSet#Equal(a,b) <==> (forall o: Box :: {a[o]} {b[o]} a[o] == b[o]));
 // extensionality axiom for multisets
 axiom (forall a: MultiSet, b: MultiSet :: { MultiSet#Equal(a,b) }
   MultiSet#Equal(a,b) ==> a == b);
 
-revealed function MultiSet#Disjoint(MultiSet, MultiSet): bool;
+function MultiSet#Disjoint(MultiSet, MultiSet): bool;
 axiom (forall a: MultiSet, b: MultiSet :: { MultiSet#Disjoint(a,b) }
   MultiSet#Disjoint(a,b) <==> (forall o: Box :: {a[o]} {b[o]} a[o] == 0 || b[o] == 0));
 
 // conversion to a multiset. each element in the original set has duplicity 1.
-revealed function MultiSet#FromSet(Set): MultiSet;
+function MultiSet#FromSet(Set): MultiSet;
 axiom (forall s: Set, a: Box :: { MultiSet#FromSet(s)[a] }
   (MultiSet#FromSet(s)[a] == 0 <==> !s[a]) &&
   (MultiSet#FromSet(s)[a] == 1 <==> s[a]));
@@ -923,7 +923,7 @@ axiom (forall s: Set :: { MultiSet#Card(MultiSet#FromSet(s)) }
   MultiSet#Card(MultiSet#FromSet(s)) == Set#Card(s));
 
 // conversion to a multiset, from a sequence.
-revealed function MultiSet#FromSeq(Seq): MultiSet uses {
+function MultiSet#FromSeq(Seq): MultiSet uses {
   axiom MultiSet#FromSeq(Seq#Empty(): Seq) == MultiSet#Empty(): MultiSet;
 }
 
@@ -960,10 +960,10 @@ axiom (forall s: Seq, x: Box :: { MultiSet#FromSeq(s)[x] }
 
 type Seq;
 
-revealed function Seq#Length(Seq): int;
+function Seq#Length(Seq): int;
 axiom (forall s: Seq :: { Seq#Length(s) } 0 <= Seq#Length(s));
 
-revealed function Seq#Empty(): Seq uses {
+function Seq#Empty(): Seq uses {
   axiom (Seq#Length(Seq#Empty(): Seq) == 0);
 }
 axiom (forall s: Seq :: { Seq#Length(s) }
@@ -978,12 +978,12 @@ axiom (forall s: Seq :: { Seq#Length(s) }
 // The empty sequence $Is any type
 //axiom (forall t: Ty :: {$Is(Seq#Empty(): Seq, TSeq(t))} $Is(Seq#Empty(): Seq, TSeq(t)));
 
-revealed function Seq#Singleton(Box): Seq;
+function Seq#Singleton(Box): Seq;
 axiom (forall t: Box :: { Seq#Length(Seq#Singleton(t)) } Seq#Length(Seq#Singleton(t)) == 1);
 
-revealed function Seq#Build(s: Seq, val: Box): Seq;
-revealed function Seq#Build_inv0(s: Seq) : Seq;
-revealed function Seq#Build_inv1(s: Seq) : Box;
+function Seq#Build(s: Seq, val: Box): Seq;
+function Seq#Build_inv0(s: Seq) : Seq;
+function Seq#Build_inv1(s: Seq) : Box;
 axiom (forall s: Seq, val: Box ::
   { Seq#Build(s, val) }
   Seq#Build_inv0(Seq#Build(s, val)) == s &&
@@ -1000,7 +1000,7 @@ axiom (forall s: Seq, i: int, v: Box :: { Seq#Index(Seq#Build(s,v), i) }
 axiom (forall s: Seq, bx: Box, t: Ty :: { $Is(Seq#Build(s,bx),TSeq(t)) }
     $Is(s,TSeq(t)) && $IsBox(bx,t) ==> $Is(Seq#Build(s,bx),TSeq(t)));
 
-revealed function Seq#Create(ty: Ty, heap: Heap, len: int, init: HandleType): Seq;
+function Seq#Create(ty: Ty, heap: Heap, len: int, init: HandleType): Seq;
 axiom (forall ty: Ty, heap: Heap, len: int, init: HandleType ::
   { Seq#Length(Seq#Create(ty, heap, len, init): Seq) }
   $IsGoodHeap(heap) && 0 <= len ==>
@@ -1010,17 +1010,17 @@ axiom (forall ty: Ty, heap: Heap, len: int, init: HandleType, i: int ::
   $IsGoodHeap(heap) && 0 <= i && i < len ==>
   Seq#Index(Seq#Create(ty, heap, len, init), i) == Apply1(TInt, ty, heap, init, $Box(i)));
 
-revealed function Seq#Append(Seq, Seq): Seq;
+function Seq#Append(Seq, Seq): Seq;
 axiom (forall s0: Seq, s1: Seq :: { Seq#Length(Seq#Append(s0,s1)) }
   Seq#Length(Seq#Append(s0,s1)) == Seq#Length(s0) + Seq#Length(s1));
 
-revealed function Seq#Index(Seq, int): Box;
+function Seq#Index(Seq, int): Box;
 axiom (forall t: Box :: { Seq#Index(Seq#Singleton(t), 0) } Seq#Index(Seq#Singleton(t), 0) == t);
 axiom (forall s0: Seq, s1: Seq, n: int :: { Seq#Index(Seq#Append(s0,s1), n) }
   (n < Seq#Length(s0) ==> Seq#Index(Seq#Append(s0,s1), n) == Seq#Index(s0, n)) &&
   (Seq#Length(s0) <= n ==> Seq#Index(Seq#Append(s0,s1), n) == Seq#Index(s1, n - Seq#Length(s0))));
 
-revealed function Seq#Update(Seq, int, Box): Seq;
+function Seq#Update(Seq, int, Box): Seq;
 axiom (forall s: Seq, i: int, v: Box :: { Seq#Length(Seq#Update(s,i,v)) }
   0 <= i && i < Seq#Length(s) ==> Seq#Length(Seq#Update(s,i,v)) == Seq#Length(s));
 axiom (forall s: Seq, i: int, v: Box, n: int :: { Seq#Index(Seq#Update(s,i,v),n) }
@@ -1028,7 +1028,7 @@ axiom (forall s: Seq, i: int, v: Box, n: int :: { Seq#Index(Seq#Update(s,i,v),n)
     (i == n ==> Seq#Index(Seq#Update(s,i,v),n) == v) &&
     (i != n ==> Seq#Index(Seq#Update(s,i,v),n) == Seq#Index(s,n)));
 
-revealed function Seq#Contains(Seq, Box): bool;
+function Seq#Contains(Seq, Box): bool;
 axiom (forall s: Seq, x: Box :: { Seq#Contains(s,x) }
   Seq#Contains(s,x) <==>
     (exists i: int :: { Seq#Index(s,i) } 0 <= i && i < Seq#Length(s) && Seq#Index(s,i) == x));
@@ -1056,7 +1056,7 @@ axiom (forall s: Seq, n: int, x: Box ::
     (exists i: int :: { Seq#Index(s, i) }
       0 <= n && n <= i && i < Seq#Length(s) && Seq#Index(s, i) == x));
 
-revealed function Seq#Equal(Seq, Seq): bool;
+function Seq#Equal(Seq, Seq): bool;
 axiom (forall s0: Seq, s1: Seq :: { Seq#Equal(s0,s1) }
   Seq#Equal(s0,s1) <==>
     Seq#Length(s0) == Seq#Length(s1) &&
@@ -1065,13 +1065,13 @@ axiom (forall s0: Seq, s1: Seq :: { Seq#Equal(s0,s1) }
 axiom (forall a: Seq, b: Seq :: { Seq#Equal(a,b) }  // extensionality axiom for sequences
   Seq#Equal(a,b) ==> a == b);
 
-revealed function Seq#SameUntil(Seq, Seq, int): bool;
+function Seq#SameUntil(Seq, Seq, int): bool;
 axiom (forall s0: Seq, s1: Seq, n: int :: { Seq#SameUntil(s0,s1,n) }
   Seq#SameUntil(s0,s1,n) <==>
     (forall j: int :: { Seq#Index(s0,j) } { Seq#Index(s1,j) }
         0 <= j && j < n ==> Seq#Index(s0,j) == Seq#Index(s1,j)));
 
-revealed function Seq#Take(s: Seq, howMany: int): Seq;
+function Seq#Take(s: Seq, howMany: int): Seq;
 axiom (forall s: Seq, n: int :: { Seq#Length(Seq#Take(s,n)) }
   0 <= n && n <= Seq#Length(s) ==> Seq#Length(Seq#Take(s,n)) == n);
 axiom (forall s: Seq, n: int, j: int ::
@@ -1081,7 +1081,7 @@ axiom (forall s: Seq, n: int, j: int ::
   0 <= j && j < n && j < Seq#Length(s) ==>
     Seq#Index(Seq#Take(s,n), j) == Seq#Index(s, j));
 
-revealed function Seq#Drop(s: Seq, howMany: int): Seq;
+function Seq#Drop(s: Seq, howMany: int): Seq;
 axiom (forall s: Seq, n: int :: { Seq#Length(Seq#Drop(s,n)) }
   0 <= n && n <= Seq#Length(s) ==> Seq#Length(Seq#Drop(s,n)) == Seq#Length(s) - n);
 axiom (forall s: Seq, n: int, j: int ::
@@ -1103,7 +1103,7 @@ axiom (forall s, t: Seq, n: int ::
   Seq#Take(Seq#Append(s, t), n) == s &&
   Seq#Drop(Seq#Append(s, t), n) == t);
 
-revealed function Seq#FromArray(h: Heap, a: ref): Seq;
+function Seq#FromArray(h: Heap, a: ref): Seq;
 axiom (forall h: Heap, a: ref ::
   { Seq#Length(Seq#FromArray(h,a)) }
   Seq#Length(Seq#FromArray(h, a)) == _System.array.Length(a));
@@ -1150,7 +1150,7 @@ axiom (forall s: Seq, v: Box, n: int ::
         { Seq#Drop(Seq#Build(s, v), n) }
         0 <= n && n <= Seq#Length(s) ==> Seq#Drop(Seq#Build(s, v), n) == Seq#Build(Seq#Drop(s, n), v) );
 
-revealed function Seq#Rank(Seq): int;
+function Seq#Rank(Seq): int;
 axiom (forall s: Seq, i: int ::
         { DtRank($Unbox(Seq#Index(s, i)): DatatypeType) }
         0 <= i && i < Seq#Length(s) ==> DtRank($Unbox(Seq#Index(s, i)): DatatypeType) < Seq#Rank(s) );
@@ -1181,11 +1181,11 @@ type Map;
 
 // A Map is defined by three functions, Map#Domain, Map#Elements, and #Map#Card.
 
-revealed function Map#Domain(Map) : Set;
+function Map#Domain(Map) : Set;
 
-revealed function Map#Elements(Map) : [Box]Box;
+function Map#Elements(Map) : [Box]Box;
 
-revealed function Map#Card(Map) : int;
+function Map#Card(Map) : int;
 
 axiom (forall m: Map :: { Map#Card(m) } 0 <= Map#Card(m));
 
@@ -1218,7 +1218,7 @@ axiom (forall m: Map ::
 // square brackets) and Map#Card, so we need to define what these mean for the Set
 // returned by Map#Values.
 
-revealed function Map#Values(Map) : Set;
+function Map#Values(Map) : Set;
 
 axiom (forall m: Map, v: Box :: { Map#Values(m)[v] }
   Map#Values(m)[v] ==
@@ -1235,11 +1235,11 @@ axiom (forall m: Map, v: Box :: { Map#Values(m)[v] }
 // definition of Map#Items here is to be considered Dafny specific.  Also, note
 // that it relies on the two destructors for 2-tuples.
 
-revealed function Map#Items(Map) : Set;
+function Map#Items(Map) : Set;
 
-revealed function #_System._tuple#2._#Make2(Box, Box) : DatatypeType;
-revealed function _System.Tuple2._0(DatatypeType) : Box;
-revealed function _System.Tuple2._1(DatatypeType) : Box;
+function #_System._tuple#2._#Make2(Box, Box) : DatatypeType;
+function _System.Tuple2._0(DatatypeType) : Box;
+function _System.Tuple2._1(DatatypeType) : Box;
 
 axiom (forall m: Map, item: Box :: { Map#Items(m)[item] }
   Map#Items(m)[item] <==>
@@ -1248,12 +1248,12 @@ axiom (forall m: Map, item: Box :: { Map#Items(m)[item] }
 
 // Here are the operations that produce Map values.
 
-revealed function Map#Empty(): Map;
+function Map#Empty(): Map;
 axiom (forall u: Box ::
         { Map#Domain(Map#Empty(): Map)[u] }
         !Map#Domain(Map#Empty(): Map)[u]);
 
-revealed function Map#Glue([Box]bool, [Box]Box, Ty): Map;
+function Map#Glue([Box]bool, [Box]Box, Ty): Map;
 axiom (forall a: [Box]bool, b: [Box]Box, t: Ty ::
   { Map#Domain(Map#Glue(a, b, t)) }
   Map#Domain(Map#Glue(a, b, t)) == a);
@@ -1269,7 +1269,7 @@ axiom (forall a: [Box]bool, b: [Box]Box, t0, t1: Ty ::
 
 
 //Build is used in displays, and for map updates
-revealed function Map#Build(Map, Box, Box): Map;
+function Map#Build(Map, Box, Box): Map;
 /*axiom (forall m: Map, u: Box, v: Box ::
   { Map#Domain(Map#Build(m, u, v))[u] } { Map#Elements(Map#Build(m, u, v))[u] }
   Map#Domain(Map#Build(m, u, v))[u] && Map#Elements(Map#Build(m, u, v))[u] == v);*/
@@ -1286,7 +1286,7 @@ axiom (forall m: Map, u: Box, v: Box :: { Map#Card(Map#Build(m, u, v)) }
   !Map#Domain(m)[u] ==> Map#Card(Map#Build(m, u, v)) == Map#Card(m) + 1);
 
 // Map operations
-revealed function Map#Merge(Map, Map): Map;
+function Map#Merge(Map, Map): Map;
 axiom (forall m: Map, n: Map ::
   { Map#Domain(Map#Merge(m, n)) }
   Map#Domain(Map#Merge(m, n)) == Set#Union(Map#Domain(m), Map#Domain(n)));
@@ -1296,7 +1296,7 @@ axiom (forall m: Map, n: Map, u: Box ::
     (!Map#Domain(n)[u] ==> Map#Elements(Map#Merge(m, n))[u] == Map#Elements(m)[u]) &&
     (Map#Domain(n)[u] ==> Map#Elements(Map#Merge(m, n))[u] == Map#Elements(n)[u]));
 
-revealed function Map#Subtract(Map, Set): Map;
+function Map#Subtract(Map, Set): Map;
 axiom (forall m: Map, s: Set ::
   { Map#Domain(Map#Subtract(m, s)) }
   Map#Domain(Map#Subtract(m, s)) == Set#Difference(Map#Domain(m), s));
@@ -1306,7 +1306,7 @@ axiom (forall m: Map, s: Set, u: Box ::
     Map#Elements(Map#Subtract(m, s))[u] == Map#Elements(m)[u]);
 
 //equality for maps
-revealed function Map#Equal(Map, Map): bool;
+function Map#Equal(Map, Map): bool;
 axiom (forall m: Map, m': Map::
   { Map#Equal(m, m') }
     Map#Equal(m, m') <==> (forall u : Box :: Map#Domain(m)[u] == Map#Domain(m')[u]) &&
@@ -1316,7 +1316,7 @@ axiom (forall m: Map, m': Map::
   { Map#Equal(m, m') }
     Map#Equal(m, m') ==> m == m');
 
-revealed function Map#Disjoint(Map, Map): bool;
+function Map#Disjoint(Map, Map): bool;
 axiom (forall m: Map, m': Map ::
   { Map#Disjoint(m, m') }
     Map#Disjoint(m, m') <==> (forall o: Box :: {Map#Domain(m)[o]} {Map#Domain(m')[o]} !Map#Domain(m)[o] || !Map#Domain(m')[o]));
@@ -1329,9 +1329,9 @@ type IMap;
 
 // A IMap is defined by two functions, Map#Domain and Map#Elements.
 
-revealed function IMap#Domain(IMap) : Set;
+function IMap#Domain(IMap) : Set;
 
-revealed function IMap#Elements(IMap) : [Box]Box;
+function IMap#Elements(IMap) : [Box]Box;
 
 axiom (forall m: IMap ::
   { IMap#Domain(m) }
@@ -1358,7 +1358,7 @@ axiom (forall m: IMap ::
 // square brackets) so we need to define what these mean for the Set
 // returned by Map#Values.
 
-revealed function IMap#Values(IMap) : Set;
+function IMap#Values(IMap) : Set;
 
 axiom (forall m: IMap, v: Box :: { IMap#Values(m)[v] }
   IMap#Values(m)[v] ==
@@ -1375,7 +1375,7 @@ axiom (forall m: IMap, v: Box :: { IMap#Values(m)[v] }
 // definition of IMap#Items here is to be considered Dafny specific.  Also, note
 // that it relies on the two destructors for 2-tuples.
 
-revealed function IMap#Items(IMap) : Set;
+function IMap#Items(IMap) : Set;
 
 axiom (forall m: IMap, item: Box :: { IMap#Items(m)[item] }
   IMap#Items(m)[item] <==>
@@ -1383,12 +1383,12 @@ axiom (forall m: IMap, item: Box :: { IMap#Items(m)[item] }
     IMap#Elements(m)[_System.Tuple2._0($Unbox(item))] == _System.Tuple2._1($Unbox(item)));
 
 // Here are the operations that produce Map values.
-revealed function IMap#Empty(): IMap;
+function IMap#Empty(): IMap;
 axiom (forall u: Box ::
         { IMap#Domain(IMap#Empty(): IMap)[u] }
         !IMap#Domain(IMap#Empty(): IMap)[u]);
 
-revealed function IMap#Glue([Box] bool, [Box]Box, Ty): IMap;
+function IMap#Glue([Box] bool, [Box]Box, Ty): IMap;
 axiom (forall a: [Box]bool, b: [Box]Box, t: Ty ::
   { IMap#Domain(IMap#Glue(a, b, t)) }
   IMap#Domain(IMap#Glue(a, b, t)) == a);
@@ -1403,7 +1403,7 @@ axiom (forall a: [Box]bool, b: [Box]Box, t0, t1: Ty ::
   $Is(Map#Glue(a, b, TIMap(t0, t1)), TIMap(t0, t1)));
 
 //Build is used in displays
-revealed function IMap#Build(IMap, Box, Box): IMap;
+function IMap#Build(IMap, Box, Box): IMap;
 /*axiom (forall m: IMap, u: Box, v: Box ::
   { IMap#Domain(IMap#Build(m, u, v))[u] } { IMap#Elements(IMap#Build(m, u, v))[u] }
   IMap#Domain(IMap#Build(m, u, v))[u] && IMap#Elements(IMap#Build(m, u, v))[u] == v);*/
@@ -1416,7 +1416,7 @@ axiom (forall m: IMap, u: Box, u': Box, v: Box ::
                IMap#Elements(IMap#Build(m, u, v))[u'] == IMap#Elements(m)[u']));
 
 //equality for imaps
-revealed function IMap#Equal(IMap, IMap): bool;
+function IMap#Equal(IMap, IMap): bool;
 axiom (forall m: IMap, m': IMap::
   { IMap#Equal(m, m') }
     IMap#Equal(m, m') <==> (forall u : Box :: IMap#Domain(m)[u] == IMap#Domain(m')[u]) &&
@@ -1427,7 +1427,7 @@ axiom (forall m: IMap, m': IMap::
     IMap#Equal(m, m') ==> m == m');
 
 // IMap operations
-revealed function IMap#Merge(IMap, IMap): IMap;
+function IMap#Merge(IMap, IMap): IMap;
 axiom (forall m: IMap, n: IMap ::
   { IMap#Domain(IMap#Merge(m, n)) }
   IMap#Domain(IMap#Merge(m, n)) == Set#Union(IMap#Domain(m), IMap#Domain(n)));
@@ -1437,7 +1437,7 @@ axiom (forall m: IMap, n: IMap, u: Box ::
     (!IMap#Domain(n)[u] ==> IMap#Elements(IMap#Merge(m, n))[u] == IMap#Elements(m)[u]) &&
     (IMap#Domain(n)[u] ==> IMap#Elements(IMap#Merge(m, n))[u] == IMap#Elements(n)[u]));
 
-revealed function IMap#Subtract(IMap, Set): IMap;
+function IMap#Subtract(IMap, Set): IMap;
 axiom (forall m: IMap, s: Set ::
   { IMap#Domain(IMap#Subtract(m, s)) }
   IMap#Domain(IMap#Subtract(m, s)) == Set#Difference(IMap#Domain(m), s));
@@ -1450,21 +1450,21 @@ axiom (forall m: IMap, s: Set, u: Box ::
 // -- Provide arithmetic wrappers to improve triggering and non-linear math
 // -------------------------------------------------------------------------
 
-revealed function INTERNAL_add_boogie(x:int, y:int) : int { x + y }
-revealed function INTERNAL_sub_boogie(x:int, y:int) : int { x - y }
-revealed function INTERNAL_mul_boogie(x:int, y:int) : int { x * y }
-revealed function INTERNAL_div_boogie(x:int, y:int) : int { x div y }
-revealed function INTERNAL_mod_boogie(x:int, y:int) : int { x mod y }
-revealed function {:never_pattern true} INTERNAL_lt_boogie(x:int, y:int) : bool { x < y }
-revealed function {:never_pattern true} INTERNAL_le_boogie(x:int, y:int) : bool { x <= y }
-revealed function {:never_pattern true} INTERNAL_gt_boogie(x:int, y:int) : bool { x > y }
-revealed function {:never_pattern true} INTERNAL_ge_boogie(x:int, y:int) : bool { x >= y }
+function INTERNAL_add_boogie(x:int, y:int) : int { x + y }
+function INTERNAL_sub_boogie(x:int, y:int) : int { x - y }
+function INTERNAL_mul_boogie(x:int, y:int) : int { x * y }
+function INTERNAL_div_boogie(x:int, y:int) : int { x div y }
+function INTERNAL_mod_boogie(x:int, y:int) : int { x mod y }
+function {:never_pattern true} INTERNAL_lt_boogie(x:int, y:int) : bool { x < y }
+function {:never_pattern true} INTERNAL_le_boogie(x:int, y:int) : bool { x <= y }
+function {:never_pattern true} INTERNAL_gt_boogie(x:int, y:int) : bool { x > y }
+function {:never_pattern true} INTERNAL_ge_boogie(x:int, y:int) : bool { x >= y }
 
-revealed function Mul(x, y: int): int { x * y }
-revealed function Div(x, y: int): int { x div y }
-revealed function Mod(x, y: int): int { x mod y }
-revealed function Add(x, y: int): int { x + y }
-revealed function Sub(x, y: int): int { x - y }
+function Mul(x, y: int): int { x * y }
+function Div(x, y: int): int { x div y }
+function Mod(x, y: int): int { x mod y }
+function Add(x, y: int): int { x + y }
+function Sub(x, y: int): int { x - y }
 
 #if ARITH_DISTR
 axiom (forall x, y, z: int ::
